concat doubly linked list

examples/lowstar_resources/LowStar.RST.DList.fst
@@ -1,4 +1,4 @@
- (*
+(*
    Copyright 2008-2019 Microsoft Research
 
    Licensed under the Apache License, Version 2.0 (the "License");
@@ -220,7 +220,7 @@ val elim_dlist_nil (#a:Type) (left:t a)
        pure (right == ptr))
 
 
-let b2p (b:bool) : prop = b == true
+
 irreducible
 let dlist_cons (#a:Type) (left:t a) 
                          (ptr:t a)
@@ -274,7 +274,6 @@ val read_ptr (#a:_) (ptr:t a) (c:cell a)
         (ensures fun _ -> pts_to ptr c)
         (requires fun _ -> True)
         (ensures fun _ c' _ -> c == c')
-    
 
 
 assume
@@ -297,6 +296,9 @@ let resource_assertion (r:resource)
         (fun _ _ _ -> True)
   = ()        
 
+#push-options "--z3rlimit_factor 20 --max_fuel 0 --initial_fuel 0 --max_ifuel 1 --initial_ifuel 1 --z3cliopt 'smt.qi.eager_threshold=100' --query_stats"
+#push-options "--log_queries"
+#restart-solver
 //#set-options "--tactic_trace_d  1"
 let new_dlist (#a:Type) (init:a)
   : Rst (t a)
@@ -305,7 +307,7 @@ let new_dlist (#a:Type) (init:a)
     (ensures fun ptr ->
       dlist null_dlist ptr null_dlist [mk_cell null_dlist null_dlist init])
   = reveal_rst_inv ();
-    reveal_modifies ();
+    // reveal_modifies ();
     reveal_empty_resource();
     reveal_star();
     let cell = mk_cell null_dlist null_dlist init in
@@ -378,7 +380,8 @@ val resource_assumption (r:resource)
         (fun _ -> True)
         (fun _ _ _ -> True)
 
-#push-options "--z3rlimit_factor 20 --max_fuel 2 --initial_fuel 2 --max_ifuel 2 --initial_ifuel 2 --z3cliopt 'smt.qi.eager_threshold=100' --query_stats"
+#restart-solver
+
 let rec concat (#a:Type)
                (from0:t a) (ptr0:t a) (to0: t a) (l0:list (cell a))
                (from1:t a) (ptr1:t a) (l1:list (cell a))
@@ -423,6 +426,7 @@ let rec concat (#a:Type)
        (fun _ -> pts_to ptr0 hd0 <*> dlist ptr0 (next hd0) to0 tl0 <*> dlist from1 ptr1 to1 l1) //<--
        (fun _ -> elim_dlist_cons from0 ptr0 to0 hd0 tl0);
 
+     let l =
      if ptr_eq (next c0) to0
      then begin //we are at the end of l0
        // 3. invert dlist tl0 to dlist []
@@ -468,11 +472,6 @@ let rec concat (#a:Type)
        intro_dlist_cons from0 ptr0 to1 c0' (c1'::tl1);
        
        let l = c0'::c1'::tl1 in       
-       resource_assertion (dlist from0 ptr0 null_dlist l);
-       let h1 = FStar.HyperStack.ST.get () in
-       assume (modifies (dlist from0 ptr0 to0 l0 <*> dlist from1 ptr1 null_dlist l1)
-                        (dlist from0 ptr0 null_dlist l) 
-                        h0 h1);
        l
      end
      else begin 
@@ -492,366 +491,14 @@ let rec concat (#a:Type)
        intro_dlist_cons from0 ptr0 null_dlist hd0 l;
        resource_assertion (dlist from0 ptr0 to1 (hd0::l));
        let l = hd0::l in
-       let h1 = FStar.HyperStack.ST.get () in
-       assume (modifies (dlist from0 ptr0 to0 l0 <*> dlist from1 ptr1 to1 l1)
-                        (dlist from0 ptr0 to1 l)
-                        h0 h1);
        l
      end
-
-     
-     
-     admit()
-       //pts_to ptr0 c1 <*> dlist to0 ptr1 to1 l1
-       //c1.next == ptr1
-       //
-       //==================================
-       //dlist from0 ptr0 to1 (c::l1)
-       
-       assert (prev c1 == from0);
-       assert (ptr0 =!= to1);
-       
-       //ptr0 <> to0
-
-       admit()
-       // if ptr_eq ptr1 to1
-       // then begin
-       //   rst_frame
-       //     (pts_to ptr0 c1 <*> dlist ptr0 to0 to0 [] <*> dlist from1 ptr1 to1 l1)
-       //     (fun _ -> pts_to ptr0 c1 <*> dlist ptr0 to0 to0 [] <*> dlist ptr0 to1 to1 [])  
-       //     (fun _ -> invert_dlist_nil_eq from1 ptr0 ptr1 to1 l1);
-  
-       //   rst_frame
-       //     (pts_to ptr0 c1 <*> dlist ptr0 to0 to0 [] <*> dlist ptr0 to1 to1 [])           
-       //     (fun _ -> pts_to ptr0 c1 <*> dlist ptr0 to0 to0 [] <*> dlist ptr0 (next c1) to1 [])
-       //     (fun _ -> rewrite_resource (dlist ptr0 to1 to1 []) (dlist ptr0 (next c1) to1 []));
-
-       //   rst_frame
-       //     (pts_to ptr0 c1 <*> dlist ptr0 to0 to0 [] <*> dlist ptr0 (next c1) to1 [])
-       //     (fun _ -> dlist from0 ptr0 to1 [c1] <*> dlist ptr0 to0 to0 [])
-       //     (fun _ -> intro_dlist_cons from0 ptr0 to1 c1 []);
-
-       //   resource_assertion (dlist from0 ptr0 to1 [c1]);
-       //   admit()
-       // end
-       // else admit()
-     end
-     else admit()
      in
+     resource_assertion (dlist from0 ptr0 null_dlist l);
      let h1 = FStar.HyperStack.ST.get () in
-     assume (modifies (dlist from0 ptr0 to0 l0 <*> dlist from1 ptr1 to1 l1)
-                      (dlist from0 ptr0 to1 (l0@l1))
+     assume (modifies (dlist from0 ptr0 to0 l0 <*> dlist from1 ptr1 null_dlist l1)
+                      (dlist from0 ptr0 null_dlist l) 
                       h0 h1);
      l
-
      
-     empty_resource (dlist null_dlist p null_dlist [cell]) h0 h1);     
-
-
-     admit()
-
-       
-     
-       let c0 = RA.index ptr0 0ul in
-       if c0.next = to0
-       then //last node in l0 ...here's where we hook it up
-            begin
-            assert (Nil? (Cons?.tl l0));
-            let _ = 
-              rst_frame
-                (dlist from0 ptr0 to0 l0 <*> dlist from1 ptr1 to1 l1)
-                (fun _ -> dlist_cons from0 ptr0 to0 l0 <*> dlist from1 ptr1 to1 l1)
-                (fun _ -> unfold_dlist_cons from0 ptr0 to0 l0)
-            in
-            // let c1 = 
-            //   rst_frame
-            //     (dlist_cons from0 ptr0 to0 l0 <*> dlist from1 ptr1 to1 l1)
-            //     (fun _ -> dlist_cons from0 ptr0 to0 l0 <*> dlist from1 ptr1 to1 l1)
-            //     (fun _ -> read_ptr ptr0 l0) in
-            admit()
-            // RA.upd c0.next 0ul c1;
-            // RA.upd c1.prev 0ul c0;
-            // admit()
-       end
-       else admit()
-            
-       
-       
-
-     // end
-     // else admit()
-
-
-// // let splice (#a:Type) (left0:t a) (ptr0:t a) (right0: t a) (l0:list a) 
-// //                      (left1:t a) (ptr1:t a) (right1: t a) (l1:list a)
-// //   : Rst unit      
-// //     (requires
-// //       dlist left0 ptr0 right0 l0 <*>
-// //       dlist left1 ptr1 right1 l1)
-
-// let make_two (#a:Type) (left:t a) (ptr:t a) (right: t a) (c0:cell a) (v:a)
-//   : RST (list (cell a))
-//     (requires
-//        dlist left ptr right [c0])
-//     (ensures fun l  ->
-//       dlist left ptr right l)
-//     (requires fun _ -> True)
-//     (ensures fun _ l _ -> 
-//       match l with 
-//       | [c0'; c1] -> c0.data == c0.data /\ c1.data == v
-//       | _ -> False)
-//   = let hd = RA.index ptr 0ul in
-//     let new_l = 
-//         new_dlist ptr v right
-//     in
-//     RA.upd hd.next 0ul new_cell
-
   
-//   admit()
-  
-// let insert_after (#a:Type) (left:t a) (ptr:t a) (right: t a{ptr =!= right)) (l:list (cell a)) (v:a)
-//   : Rst unit
-//     (requires 
-//       dlist left ptr right l)
-//     (ensures fun _ -> 
-//       let hd::tl = l in
-//       let new_cell = {
-//           data = init;
-//        }
-//       in
-//       dlist left ptr right (hd::
-//       empty_resource)
-//       // let c_v = { data = v; prev = left; next = ptr} in
-//       // dlist left ptr right (c_v :: l))
-//   = reveal_rst_inv ();
-//     reveal_modifies ();
-//     reveal_empty_resource();
-//     reveal_star();
-//     let hd = RA.index ptr 0ul in
-//     let new_cell = 
-//            RA.alloc ({
-//              data = init;
-//              prev = ptr;
-//              next = hd.next;
-//            })
-//     in
-//     RA.upd ptr.next 0ul new_cell;
-//     if hd.next = right then ()
-//     else begin
-//       admit();
-//       let next_cell = RA.index hd.next 0ul in
-//       RA.upd next_cell.prev 0ul new_cell
-//     end
-
-
-          
-//            new_dlist init in
-//          RA.upd new_cell.prev :=
-    
-//       dlist null_dlist ptr null_dlist [{prev = null_dlist;
-//                                         next = null_dlist;
-//                                         data = init}])
-
-
-
-
-// abstract
-// let dummy_cell (#a:Type) (ptr:t a) : resource =
-//   hsrefine (RA.array_resource ptr) node_inv
-
-// let cell_alloc (#a:Type)
-//               (init:cell a)
-//             : RST (t a) (empty_resource)
-//                         (fun ptr -> pts_to ptr init)
-//                         (fun _ -> True)
-//                         (fun _ ptr h1 -> True) =
-//   reveal_rst_inv ();
-//   reveal_modifies ();
-//   RA.alloc init 1ul
-
-
-// let cell_free (#a:Type)
-//               (ptr:t a)
-//               (v:cell a)
-//            : RST unit (pts_to ptr v)
-//                       (fun ptr -> empty_resource)
-//                       (fun _ -> True)
-//                       (fun _ ptr h1 -> True) =
-//   reveal_rst_inv ();
-//   reveal_modifies ();
-//   reveal_empty_resource ();
-//   RA.free ptr
-
-// let set_dummy_cell (#a:Type) (ptr:t a) (c:cell a)
-//   : RST unit
-//     (dummy_cell ptr)
-//     (fun _ -> pts_to ptr c)
-//     (fun _ -> True)
-//     (fun _ _ _ -> True)
-//   = reveal_rst_inv();
-//     reveal_modifies();
-//     RA.upd ptr 0ul c
-
-// let set_cell (#a:Type) (ptr:t a) (c:cell a) (v:a)
-//   : RST unit
-//     (pts_to ptr c)
-//     (fun _ -> pts_to ptr ({c with data = v}))
-//     (fun _ -> True)
-//     (fun _ _ _ -> True)
-//   = reveal_rst_inv();
-//     reveal_modifies();
-//     let h0 = HyperStack.ST.get() in
-//     let node = RA.index ptr 0ul in
-//     let node' = {node with data = v} in
-//     let h0' = HyperStack.ST.get() in
-//     RA.upd ptr 0ul node';
-//     let h1 = HyperStack.ST.get() in
-//     // Unclear why modifies_trans does not trigger automatically
-//     assert (modifies (pts_to ptr c) (pts_to ptr c) h0 h0');
-//     assert (modifies (pts_to ptr c) (pts_to ptr node') h0' h1)
-
-// #reset-options "--z3rlimit 20 --max_fuel 1 --max_ifuel 1 --z3cliopt smt.QI.EAGER_THRESHOLD=2"
-
-// (* We provide two versions of cons.
-//    The first one assumes there is an unused (dummy) node, that we can just set to be the head.
-//    The second performs an allocation *)
-
-// let cons (#a:Type) (ptr:t a) (l:list (cell a)) (h:t a) (v:a) (x:a)
-//   : RST unit
-//   (dummy_cell h <*> slist ptr l)
-//   (fun _ -> slist h ({data = v; next = ptr} :: l))
-//   (fun _ -> True)
-//   (fun _ _ _ -> True) =
-//   let new_cell = {data = v; next = ptr} in
-//   rst_frame
-//     (dummy_cell h <*> slist ptr l)
-//     (fun _ -> pts_to h new_cell <*> slist ptr l)
-//     (fun _ -> set_dummy_cell h new_cell)
-
-// let cons_alloc (#a:Type) (ptr:t a) (l:list (cell a)) (v:a)
-//   : RST (t a)
-//   (slist ptr l)
-//   (fun ptr' -> slist ptr' ({data = v; next = ptr} :: l))
-//   (fun _ -> True)
-//   (fun _ _ _ -> True) =
-//   let new_cell = {data = v; next = ptr} in
-//   let new_head = rst_frame
-//     (slist ptr l)
-//     #_ #_
-//     (fun ret -> pts_to ret new_cell <*> slist ptr l)
-//     #_
-//     #(slist ptr l)
-//     (fun _ -> cell_alloc new_cell)
-//   in
-//   new_head
-
-// (* Similarly, we provide two versions of uncons.
-//    The second deallocates the node currently in head position, while the first
-//    returns the head and the tail *)
-
-// let uncons (#a:Type) (ptr:t a) (l:list (cell a){Cons? l})
-//   : RST (t a * t a)
-//         (slist ptr l)
-//         (fun (hd, ptr') -> pts_to hd (L.hd l) <*> slist ptr' (L.tl l))
-//         (requires fun _ -> True)
-//         (ensures fun _ _ _ -> True)
-//   =
-//   RA.reveal_array();
-//   let node = LowStar.Array.index ptr 0ul in
-//   let next = node.next in
-//   ptr, next
-
-// let uncons_dealloc (#a:Type) (ptr:t a) (l:list (cell a){Cons? l})
-//   : RST (t a)
-//         (slist ptr l)
-//         (fun ptr' -> slist ptr' (L.tl l))
-//         (requires fun _ -> True)
-//         (ensures fun _ _ _ -> True)
-//   =
-//   RA.reveal_array();
-//   let node = LowStar.Array.index ptr 0ul in
-//   let next = node.next in
-//   rst_frame
-//     (pts_to ptr (L.hd l) <*> slist next (L.tl l))
-//     (fun _ -> slist next (L.tl l))
-//     (fun _ -> cell_free ptr (L.hd l));
-//   next
-
-// val map (#a:Type) (f:a -> a) (ptr:t a) (l:list (cell a))
-//   : RST unit
-//         (slist ptr l)
-//         (fun _ -> slist ptr (L.map (fun x -> ({x with data = f x.data})) l))
-//         (requires fun _ -> True)
-//         (ensures fun _ _ _ -> True)
-
-
-// // LowStar.Array does not yet have a notion of null pointers. In the meantime, we assume this
-// // stateful function. It is currently incorrect as it should be y <==> g_is_null b, 
-// // and we will also need to change the definition of an empty node to a null array
-// assume
-// val is_null (#a:Type0) (b:LowStar.Array.array a)
-//   :HyperStack.ST.Stack bool (requires (fun h -> A.live h b))
-//                   (ensures  fun h y h' -> h == h' /\ (y <==> A.vlength b == 0))
-
-// let rec map #a f ptr l =
-//   RA.reveal_array();
-//   let h0 = HyperStack.ST.get() in
-//   if is_null ptr then ()
-//   else (
-//     let node = LowStar.Array.index ptr 0ul in
-//     let next = node.next in
-//     let l_tl = L.tl l in
-//     rst_frame
-//       (pts_to ptr node <*> slist next l_tl)
-//       (fun _ -> pts_to ptr ({node with data = f node.data}) <*> slist next l_tl)
-//       (fun _ -> set_cell ptr node (f node.data));
-//     rst_frame
-//       (pts_to ptr ({node with data = f node.data}) <*> slist next l_tl)
-//       (fun _ -> pts_to ptr ({node with data = f node.data}) <*>
-//              slist next (L.map (fun x -> ({x with data = f x.data})) l_tl))
-//       (fun _ -> map f next l_tl)
-//   )
-
-// type llist (a: Type0) = t a & list (cell a)
-
-// let llist_resource (#a:Type0) (x:llist a) =
-//   slist (fst x) (snd x)
-
-// let rec llist_view_aux (#a:Type0) (x:list (cell a)) : list a =
-//   match x with
-//   | [] -> []
-//   | hd::tl -> hd.data :: llist_view_aux tl
-
-// let llist_view (#a:Type0) (x:llist a) : list a =
-//   llist_view_aux (snd x)
-
-// let llist_cons #a x v =
-//   let init_ptr = fst x in
-//   let init_l = snd x in
-//   let ptr = cons_alloc init_ptr init_l v in
-//   (ptr, ({data = v; next = init_ptr} :: init_l))
-
-// let llist_head #a x =
-//   RA.reveal_array();
-//   let init_ptr = fst x in
-//   let node = LowStar.Array.index init_ptr 0ul in
-//   node.data
-
-// let llist_tail #a x =
-//   let init_ptr = fst x in
-//   let init_l = snd x in
-//   (uncons_dealloc init_ptr init_l, L.tl init_l)
-
-// let rec lemma_map_view_aux (#a:Type0) (f:a -> a) (init_l:list (cell a))
-//   : Lemma (llist_view_aux (L.map (fun x -> ({x with data = f x.data})) init_l) ==
-//           L.map f (llist_view_aux init_l))
-//    = match init_l with
-//   | [] -> ()
-//   | hd :: tl -> lemma_map_view_aux f tl
-
-// let llist_map #a f x =
-//   let init_ptr = fst x in
-//   let init_l = snd x in
-//   map f init_ptr init_l;
-//   lemma_map_view_aux f init_l;
-//   (init_ptr, L.map (fun x -> ({x with data = f x.data})) init_l)
